Example.thy
@@ -31,27 +31,105 @@ thm hnr_uRETURN_pass
 lemma moneq: "(\<lambda>s. RETURNT (0 < s)) = (\<lambda>s. RETURNT 0 \<bind> (%c. RETURNT (c < s)))"
   by (auto intro!: pw_eqI)
 
-schematic_goal
+lemma moneq_min: "(\<lambda>s. RETURNT (s - 1)) = (\<lambda>s. RETURNT 1 \<bind> (%c. RETURNT (s - c)))"
+  by (auto intro!: pw_eqI)
+
+lemma x0: "RETURNT x \<le> RETURNT 0 \<longleftrightarrow> x=0"
+  by (auto simp: RETURNT_def le_fun_def split: if_splits)  
+
+lemma [simp]: "h\<Turnstile>\<up>b \<longleftrightarrow> (h\<Turnstile>emp \<and> b)" 
+  using one_assn_rule pure_assn_rule by auto 
+
+lemma zuf: "\<up> True * true =  true"  
+  by (simp add: abel_semigroup.commute assn_ext mult.abel_semigroup_axioms)  
+
+lemma hn_refine_less: " hn_refine (hn_val nat_rel s' s * hn_val nat_rel x' x)
+           (ureturn (x < s))
+       (hn_val nat_rel s' s * hn_val nat_rel x' x)
+       (pure bool_rel) (RETURNT (x' < s'))"
+  unfolding hn_refine_def apply (auto simp: zuf mult.assoc  execute_ureturn pure_def hn_ctxt_def)
+   apply(rule exI[where x=0]) apply (auto simp: zero_enat_def relH_def )      
+    using models_in_range top_assn_rule by blast 
+
+
+lemma hn_refine_minus: " hn_refine (hn_val nat_rel s' s * hn_val nat_rel x' x)
+           (ureturn (x - s))
+       (hn_val nat_rel s' s * hn_val nat_rel x' x)
+       (pure nat_rel) (RETURNT (x' - s'))"
+  unfolding hn_refine_def apply (auto simp: zuf mult.assoc  execute_ureturn pure_def hn_ctxt_def)
+   apply(rule exI[where x=0]) apply (auto simp: zero_enat_def relH_def )      
+    using models_in_range top_assn_rule by blast 
+
+
+schematic_goal first:
   assumes "a = (whileT (\<lambda>s. s>0) (\<lambda>s. RETURNT (s-1)) (S::nat))"
   shows "hn_refine emp ?c ?\<Gamma> (pure Id) a"
   unfolding assms 
-  apply(subst WHILEIT_to_monadic) apply(subst moneq)
+  apply(subst whileT_I')
+  apply(subst WHILEIT_to_monadic) apply(subst moneq)  apply(subst moneq_min)
   apply(rule hn_monadic_WHILE_aux[where \<Gamma>="emp"])
       apply (simp add: hn_ctxt_def pure_def k entailst_def ) 
   
      apply (simp del: nres_bind_left_identity)
-     apply(rule hnr_bind) 
+     apply(rule hnr_bind)  
+     apply(rule hnr_frame)   
+        apply(rule hnr_uRETURN_pure[where R=nat_rel]) apply simp
+       apply (simp add: ) apply(rule entt_refl)
+      apply (simp  )  
+      apply(rule hn_refine_less)
+  apply(simp add: mult.assoc)
+  apply(rule match_first) 
+     apply(rule match_rest) apply (simp)
 
-     apply(rule hn_refine_cons_pre)
-      prefer 2     
-     apply(rule hnr_uRETURN_pass)
-     apply simp
-  apply (simp add: hn_ctxt_def pure_def k) 
-  using hnr_uRETURN_pass
-  using hnr_uRETURN_pure
-  subgoal unfolding hn_ctxt_def
-  apply(rule hnr_uRETURN_pure)
+  apply(simp add: entailst_def)
+    apply(rule match_rest) apply (simp)
+
+   apply (simp del: nres_bind_left_identity)
+     apply(rule hnr_bind)  
+     apply(rule hnr_frame)   
+        apply(rule hnr_uRETURN_pure[where R=nat_rel]) apply simp
+       apply (simp add: ) apply(rule entt_refl)
+      apply (simp  )  
+     apply(rule hn_refine_cons_pre[OF _ hn_refine_minus])
+  apply(simp add: entailst_def)
+    apply rotatel apply(rule match_first)   apply(rule match_rest) apply simp
+   apply rotatel apply(rule match_first) apply (rule match_rest) apply simp
   
+  apply (simp add: hn_ctxt_def pure_def k)  
+  by (simp add: ent_imp_entt)  
+
+thm first extract_cost_ub hnr_refine
+
+
+lemma entails_ex': "((\<exists>\<^sub>Ax. P x) \<Longrightarrow>\<^sub>A Q) \<longleftrightarrow> (\<forall>x. (P x \<Longrightarrow>\<^sub>A Q))"
+  using entails_ex by blast
+
+thm ex4_ref ex4'
+schematic_goal "S \<le> n \<Longrightarrow> <$ n> (heap_WHILET (\<lambda>s. ureturn 0 \<bind> (\<lambda>x'. ureturn (x' < s))) (\<lambda>s. ureturn (Suc 0) \<bind> (\<lambda>x'. ureturn (s - x'))) S) <\<lambda>r. \<up> (r = 0)>\<^sub>t"
+proof -
+  assume as: "S \<le> n"
+  from ex4_ref have "whileT (op < 0) (\<lambda>s. RETURNT (s - 1)) S \<le> whileT (op < 0) (\<lambda>s. SPECT [s - 1 \<mapsto> 1]) S" by auto
+  also from as ex4' have "\<dots> \<le> SPECT (\<lambda>s. if s = 0 then Some (enat n) else None) " by simp
+  finally have spec: "whileT (op < 0) (\<lambda>s. RETURNT (s - 1)) S \<le> SPECT (\<lambda>s. if s = 0 then Some (enat n) else None)" .
+
+  let ?P= "(heap_WHILET (\<lambda>s. ureturn 0 \<bind> (\<lambda>x'. ureturn (x' < s))) (\<lambda>s. ureturn (Suc 0) \<bind> (\<lambda>x'. ureturn (s - x'))) S)"
+  from hnr_refine[OF spec first] have "hn_refine emp ?P (emp * hn_invalid (pure nat_rel) S S) (pure nat_rel)
+   (SPECT (\<lambda>s. if s = 0 then Some (enat n) else None))" by auto
+
+  from extract_cost_ub[OF this, where Cost_ub=n] have "< $ n> ?P <\<lambda>r. emp * hn_invalid (pure nat_rel) S S * (\<exists>\<^sub>Ara. pure nat_rel ra r * \<up> (ra \<in> dom (\<lambda>s. if s = 0 then Some (enat n) else None)))>\<^sub>t"
+    by simp
+  then show "<$ n> ?P <\<lambda>r. \<up> (r = 0)>\<^sub>t"
+      apply(rule post_rule)
+    apply (simp add: pure_def hn_ctxt_def invalid_assn_def)
+       apply (auto simp: )
+    apply rotatel apply rotatel apply(simp add: ex_distrib_star[symmetric] entails_ex'  )
+    apply auto  
+    by (smt SepAuto.mod_pure_star_dist abel_semigroup.commute entails_def entails_true mult.abel_semigroup_axioms pure_conj)
+qed
+  
+
+
+thm hnr_refine[OF _ first]
 
 
 end
