Tools.thy
@@ -24,14 +24,14 @@ subsection "Rotate method"
 
 
 
-lemma left_move_back: "(A \<Longrightarrow>\<^sub>A B * C) \<Longrightarrow> (A \<Longrightarrow>\<^sub>A C * B)"
+lemma right_move_back: "(A \<Longrightarrow>\<^sub>A B * C) \<Longrightarrow> (A \<Longrightarrow>\<^sub>A C * B)"
   by (simp add: assn_times_comm)
-lemma right_move_back: "(B * C \<Longrightarrow>\<^sub>A A) \<Longrightarrow> (C * B \<Longrightarrow>\<^sub>A A)"
+lemma left_move_back: "(B * C \<Longrightarrow>\<^sub>A A) \<Longrightarrow> (C * B \<Longrightarrow>\<^sub>A A)"
   by (simp add: assn_times_comm)
 
 thm mult.assoc
-method rotater = ( (simp add: mult.assoc)? , rule left_move_back , (simp add: mult.assoc)?  )
-method rotatel = ( (simp add: mult.assoc)? , rule right_move_back , (simp add: mult.assoc)?  )
+method rotater = ( (simp add: mult.assoc)? , rule right_move_back , (simp add: mult.assoc)?  )
+method rotatel = ( (simp add: mult.assoc)? , rule left_move_back , (simp add: mult.assoc)?  )
 
 lemma "\<And>x y. A \<Longrightarrow>\<^sub>A B x y * C"
   apply rotater
@@ -126,6 +126,79 @@ method_setup weaken_hnr_post = \<open>Scan.succeed (fn ctxt => SIMPLE_METHOD'  (
   \<open>Convert "hn_invalid" to "hn_ctxt (\<lambda>_ _. true)" in postcondition of hn_refine goal\<close>
 
 
+
+subsection "refine setup"
+
+ML \<open>
+  structure refine = Named_Thms
+    ( val name = @{binding refine}
+      val description = "Refinement Framework: Refinement rules (intro)" )\<close>
+
+ML {*
+structure Refine = struct
+
+  structure vcg = Named_Thms
+    ( val name = @{binding refine_vcg}
+      val description = "Refinement Framework: " ^ 
+        "Verification condition generation rules (intro)" )
+
+  structure vcg_cons = Named_Thms
+    ( val name = @{binding refine_vcg_cons}
+      val description = "Refinement Framework: " ^
+        "Consequence rules tried by VCG" )
+
+  structure refine0 = Named_Thms
+    ( val name = @{binding refine0}
+      val description = "Refinement Framework: " ^
+        "Refinement rules applied first (intro)" )
+
+  structure refine = Named_Thms
+    ( val name = @{binding refine}
+      val description = "Refinement Framework: Refinement rules (intro)" )
+
+  structure refine2 = Named_Thms
+    ( val name = @{binding refine2}
+      val description = "Refinement Framework: " ^
+        "Refinement rules 2nd stage (intro)" )
+
+  (* If set to true, the product splitter of refine_rcg is disabled. *)
+  val no_prod_split = 
+    Attrib.setup_config_bool @{binding refine_no_prod_split} (K false);
+
+  fun rcg_tac add_thms ctxt = 
+    let 
+      val cons_thms = vcg_cons.get ctxt
+      val ref_thms = (refine0.get ctxt 
+        @ add_thms @ refine.get ctxt @ refine2.get ctxt);
+      val prod_ss = (Splitter.add_split @{thm prod.split} 
+        (put_simpset HOL_basic_ss ctxt));
+      val prod_simp_tac = 
+        if Config.get ctxt no_prod_split then 
+          K no_tac
+        else
+          (simp_tac prod_ss THEN' 
+            REPEAT_ALL_NEW (resolve_tac ctxt @{thms impI allI}));
+    in
+      REPEAT_ALL_NEW_FWD (DETERM o FIRST' [
+        resolve_tac ctxt ref_thms,
+        resolve_tac ctxt cons_thms THEN' resolve_tac ctxt ref_thms,
+        prod_simp_tac
+      ])
+    end;
+
+  fun post_tac ctxt = REPEAT_ALL_NEW_FWD (FIRST' [
+    eq_assume_tac,
+    (*match_tac ctxt thms,*)
+    SOLVED' (Tagged_Solver.solve_tac ctxt)]) 
+         
+
+end;
+*}
+setup {* Refine.vcg.setup *}
+setup {* Refine.vcg_cons.setup *}
+setup {* Refine.refine0.setup *}
+setup {* Refine.refine.setup *}
+setup {* Refine.refine2.setup *}
 
 
 end
